src/Dafny/util/pow.dfy
@@ -8,27 +8,19 @@ ensures 1 <= x ==> 1 <= p
     if k == 0 then 1 else x * pow(x,k-1)
 }
 
-lemma {:induction k} pow_0(k: nat)
-ensures 0 <= pow(0, k) <= 1
-{
-}
-
 lemma {:induction k1} pow_plus(x: nat, k1: nat, k2: nat)
 ensures pow(x, k1) * pow(x, k2) == pow(x, k1+k2)
-{
-}
+{}
 
 lemma {:induction k} pow_pos(x: nat, k: nat)
 requires 0 < x
 ensures 0 < pow(x, k)
-{
-}
+{}
 
-lemma {:induction x2} mul_increasing(x1: nat, x2: nat)
+lemma mul_increasing(x1: nat, x2: nat)
 requires 0 < x2
 ensures x1 <= x1 * x2
-{
-}
+{}
 
 lemma {:induction k1} pow_increasing(x: nat, k1: nat, k2: nat)
 requires 0 < x
